update to strengthening actual lemmas

type_members/ftfjp2018/coq/vars.v
@@ -7,12 +7,40 @@ Require Import CpdtTactics.
 Require Import definitions.
 Require Import common.
 Require Import weakening.
-Require Import subst.
 Require Import strengthening.
+Require Import subst.
 Set Implicit Arguments.
 
-Lemma wf_contains_implies_contains :
-  (forall Sig G t s, Sig en G vdash s cont_w t ->
+
+Reserved Notation "Sig 'en' G 'vdash' p 'ni_w' s" (at level 80).
+Reserved Notation "s 'cont_w' t" (at level 80).
+
+
+Inductive struct_contains : ty -> decl_ty -> Prop :=
+| cont_wf : forall ss s, in_dty s ss ->
+                    s cont_w (str ss)
+where "s 'cont_w' t" := (struct_contains t s).
+
+
+Inductive alt_has : env -> env -> exp -> decl_ty -> Prop :=
+| h_struct : forall Sig G p ss s, Sig en G vdash p pathType (str ss) ->
+                           s cont_w (str ss) ->
+                           Sig en G vdash p ni_w ([p /s 0] s)
+| h_upper : forall Sig G p p' l' t s, Sig en G vdash p pathType (sel p' l') ->
+                               Sig en G vdash p' ni_w (type l' ext t) ->
+                               Sig en G vdash (p cast t) ni_w s ->
+                               Sig en G vdash p ni_w s
+| h_equal : forall Sig G p p' l' t s, Sig en G vdash p pathType (sel p' l') ->
+                               Sig en G vdash p' ni_w (type l' eqt t) ->
+                               Sig en G vdash (p cast t) ni_w s ->
+                               Sig en G vdash p ni_w s
+where "Sig 'en' G 'vdash' p 'ni_w' s" := (alt_has Sig G p s).
+
+
+Hint Constructors alt_has struct_contains.
+
+Lemma struct_contains_implies_contains :
+  (forall Sig G t s, s cont_w t ->
               Sig en G vdash s cont t).
 Proof.
   intros;
@@ -32,49 +60,222 @@ Qed.
 
 Hint Resolve path_typing_is_path.
 
-Lemma bleh :
-  (forall Sig G p s, Sig en G vdash p ni_w s ->
-              forall t, Sig en G vdash p pathType t ->
-                   closed_exp p 0 ->
-                   closed_ty t 0 ->
-                   closed_env G 0 ->
-                   closed_env Sig 0 ->
-                   exists s', Sig en G vdash s' cont t /\
-                         s = ([p /s 0] s')).
+Lemma closed_struct_contains :
+  forall s t n, s cont_w t ->
+           closed_ty t n ->
+           closed_decl_ty s (S n).
 Proof.
-  intros Sig G p s Hni;
-    induction Hni;
+  intros.
+  inversion H; subst.
+  apply closed_in_dty with (ss:=ss);
+    auto.
+  eapply closed_ty_str; eauto.
+Qed.
+
+Lemma closed_alt_has :
+  forall Sig G p s, Sig en G vdash p ni_w s ->
+             closed_exp p 0 ->
+             closed_env Sig 0 ->
+             closed_env G 0 ->
+             closed_decl_ty s 0.
+Proof.
+  intros Sig G p s Hhas;
+    induction Hhas;
     intros.
 
   (*struct*)
-  exists s;
-    split; auto.
-  apply wf_contains_implies_contains;
+  apply closed_subst_hole_decl_ty;
     auto.
-  apply path_typing_uniqueness with (t:=str ss) in H1;
-    auto;
-    subst t;
-    auto.
+  eapply closed_struct_contains;
+    eauto.
+  eapply closed_typing_p;
+    eauto.
 
   (*upper*)
-  destruct IHHni2
-    with
-      (t0:=t)
-    as [s' Ha];
+  apply IHHhas2;
     auto.
+  apply closed_exp_cast;
+    split;
+    auto.
+  apply closed_decl_ty_upper
+    with (L:=l').
+  apply IHHhas1;
+    auto.
+  eapply closed_ty_sel with (l:=l'); eauto.
+  eapply closed_typing_p; eauto.
 
-  apply pt_cast; eauto.
-  apply closed_typing_p with (m:=0) in H;
+  (*equal*)
+  apply IHHhas2;
     auto.
-  eapply closed_exp_cast; split; eauto.
-  
-  
+  apply closed_exp_cast;
+    split;
+    auto.
+  apply closed_decl_ty_equal
+    with (L:=l').
+  apply IHHhas1;
+    auto.
+  eapply closed_ty_sel with (l:=l'); eauto.
+  eapply closed_typing_p; eauto.
 Qed.
 
+Lemma raise_n_0 :
+  forall n, (n raise_n 0) = S n.
+Proof.
+  intros;
+    unfold raise_nat;
+    assert (Hnlt : ~ n < 0);
+    [crush
+    |apply Nat.ltb_nlt in Hnlt;
+     rewrite Hnlt;
+     rewrite Nat.add_1_r;
+     auto].
+Qed.
+
+Lemma subst_same_mutind :
+  (forall t p1 p2 n, ([p1 /t n]([p2 /t n] t)) = ([[p1 /e n] p2 /t n] t)) /\
+
+  (forall s p1 p2 n, ([p1 /s n]([p2 /s n] s)) = ([[p1 /e n] p2 /s n] s)) /\
+
+  (forall ss p1 p2 n, ([p1 /ss n]([p2 /ss n] ss)) = ([[p1 /e n] p2 /ss n] ss)) /\
+
+  (forall e p1 p2 n, ([p1 /e n]([p2 /e n] e)) = ([[p1 /e n] p2 /e n] e)) /\
+
+  (forall d p1 p2 n, ([p1 /d n]([p2 /d n] d)) = ([[p1 /e n] p2 /d n] d)) /\
+
+  (forall ds p1 p2 n, ([p1 /ds n]([p2 /ds n] ds)) = ([[p1 /e n] p2 /ds n] ds)).
+Proof.
+  apply type_exp_mutind; intros; auto;
+    try solve [simpl;
+               rewrite H;
+               try (rewrite H0);
+               try (rewrite H1);
+               try (rewrite raise_subst_distr_exp);
+               try (rewrite raise_n_0);
+               auto].
+
+  destruct v as [x|x];
+    simpl; auto.
+  destruct (Nat.eq_dec n x) as [Heq|Heq];
+    [subst;
+     rewrite <- beq_nat_refl;
+     auto
+    |apply Nat.eqb_neq in Heq;
+     rewrite Heq;
+     simpl;
+     rewrite Heq;
+     auto].
+Qed.
+
+Lemma subst_same_type :
+  (forall t p1 p2 n, ([p1 /t n]([p2 /t n] t)) = ([[p1 /e n] p2 /t n] t)).
+Proof.
+  destruct subst_same_mutind; crush.
+Qed.
+
+Lemma subst_same_decl_ty :
+  (forall s p1 p2 n, ([p1 /s n]([p2 /s n] s)) = ([[p1 /e n] p2 /s n] s)).
+Proof.
+  destruct subst_same_mutind; crush.
+Qed.
+
+Lemma subst_same_var_decl_tys :
+  (forall ss p1 p2 n, ([p1 /ss n]([p2 /ss n] ss)) = ([[p1 /e n] p2 /ss n] ss)).
+Proof.
+  destruct subst_same_mutind; crush.
+Qed.
+
+Lemma subst_same_exp :
+  (forall e p1 p2 n, ([p1 /e n]([p2 /e n] e)) = ([[p1 /e n] p2 /e n] e)).
+Proof.
+  destruct subst_same_mutind; crush.
+Qed.
+
+Lemma subst_same_decl :
+  (forall d p1 p2 n, ([p1 /d n]([p2 /d n] d)) = ([[p1 /e n] p2 /d n] d)).
+Proof.
+  destruct subst_same_mutind; crush.
+Qed.
+
+Lemma subst_same_var_decls :
+  (forall ds p1 p2 n, ([p1 /ds n]([p2 /ds n] ds)) = ([[p1 /e n] p2 /ds n] ds)).
+Proof.
+  destruct subst_same_mutind; crush.
+Qed.
+
+Lemma has_contains_equivalence_mutind :
+  (forall Sig G p s, Sig en G vdash p ni s ->
+              closed_exp p 0 ->
+              closed_decl_ty s 0 ->
+              closed_env G 0 ->
+              closed_env Sig 0 ->
+              Sig en G vdash p ni_w s) /\
+  (forall Sig G t s, Sig en G vdash s cont t ->
+              forall p, Sig en G vdash p pathType t ->
+                   closed_ty t 0 ->
+                   closed_env G 0 ->
+                   closed_env Sig 0 ->
+                   Sig en G vdash p ni_w ([p /s 0]s)).
+Proof.
+  apply has_contains_mutind;
+    intros.
+
+  (*has path*)
+  apply H;
+    auto.
+  eapply closed_typing_p;
+    eauto.
   
-Lemma wf_has_implies_has :
-  (forall Sig G p s, Sig en G vdash p ni_w s ->
-              Sig en G vdash p ni s).
+  (*cont struct*)
+  eapply h_struct;
+    eauto.
+
+  (*cont upper*)
+  assert (Hclosed_p : closed_exp p 0);
+    [eapply closed_ty_sel;
+     eauto
+    |].
+  assert (Hclosed_Lt : closed_decl_ty (type L ext t) 0);
+    [eapply closed_has;
+     eauto
+    |].
+  assert (Hclosed_t : closed_ty t 0);
+    [eapply closed_decl_ty_upper;
+     eauto
+    |].
+  rewrite subst_same_decl_ty.
+  simpl.
+  rewrite closed_subst_type;
+    auto.
+  eapply h_upper;
+    eauto.
+
+  (*equal*)
+  assert (Hclosed_p : closed_exp p 0);
+    [eapply closed_ty_sel;
+     eauto
+    |].
+  assert (Hclosed_Lt : closed_decl_ty (type L eqt t) 0);
+    [eapply closed_has;
+     eauto
+    |].
+  assert (Hclosed_t : closed_ty t 0);
+    [eapply closed_decl_ty_equal;
+     eauto
+    |].
+  rewrite subst_same_decl_ty.
+  simpl.
+  rewrite closed_subst_type;
+    auto.
+  eapply h_equal;
+    eauto.
+Qed.
+
+Lemma alt_has_implies_has :
+  forall Sig G p s, Sig en G vdash p ni_w s ->
+             closed_exp p 0 ->
+             closed_env Sig 0 ->
+             closed_env G 0 ->
+             Sig en G vdash p ni s.
 Proof.
   intros Sig G p s Hni;
     induction Hni;
@@ -84,10 +285,122 @@ Proof.
   (*struct*)
   apply has_path with (t:=str ss);
     auto.
-  apply wf_contains_implies_contains;
+  apply struct_contains_implies_contains;
     auto.
 
   (*upper*)
+  assert (Hclosed_p' : closed_exp p' 0);
+    [eapply closed_ty_sel;
+     eapply closed_typing_p;
+     eauto|].
+  assert (Hclosed_lt : closed_decl_ty (type l' ext t) 0);
+    [eapply closed_alt_has;
+     eauto|].
+  assert (Hclosed_t : closed_ty t 0);
+    [eapply closed_decl_ty_upper;
+     eauto|].
+  assert (Hhas1 : Sig en G vdash p cast t ni s);
+    [apply IHHni2;
+     auto;
+     eapply closed_exp_cast;
+     eauto|].
+    inversion Hhas1;
+    subst.
+  inversion H3;
+    subst t0;
+    subst.
+  assert (Hrewrite1 : (p cast t) = ([p /e 0]((a_ 0) cast t)));
+    [simpl;
+     rewrite closed_subst_type;
+     auto
+    |rewrite Hrewrite1;
+     rewrite <- subst_same_decl_ty].
+  apply has_path with (t:=sel p' l');
+  auto.
+
+  (*equal*)
+  assert (Hclosed_p' : closed_exp p' 0);
+    [eapply closed_ty_sel;
+     eapply closed_typing_p;
+     eauto|].
+  assert (Hclosed_lt : closed_decl_ty (type l' eqt t) 0);
+    [eapply closed_alt_has;
+     eauto|].
+  assert (Hclosed_t : closed_ty t 0);
+    [eapply closed_decl_ty_equal;
+     eauto|].
+  assert (Hhas1 : Sig en G vdash p cast t ni s);
+    [apply IHHni2;
+     auto;
+     eapply closed_exp_cast;
+     eauto|].
+    inversion Hhas1;
+    subst.
+  inversion H3;
+    subst t0;
+    subst.
+  assert (Hrewrite1 : (p cast t) = ([p /e 0]((a_ 0) cast t)));
+    [simpl;
+     rewrite closed_subst_type;
+     auto
+    |rewrite Hrewrite1;
+     rewrite <- subst_same_decl_ty].
+  apply has_path with (t:=sel p' l');
+  auto.
+Qed.
+
+Lemma in_dty_wf :
+  forall s ss, in_dty s ss ->
+          forall Sig G, Sig en G vdash ss wf_ss ->
+                 Sig en G vdash s wf_s.
+Proof.
+  intros s ss Hin;
+    induction Hin;
+    intros;
+    auto;
+    inversion H;
+    subst;
+    auto.
+Qed.
+
+Lemma subst_in_dty :
+  forall s ss, in_dty s ss ->
+          forall p n, in_dty ([p /s n] s) ([p /ss n]ss).
+Proof.
+  intros s ss Hin;
+    induction Hin;
+    intros;
+    auto.
+
+  apply in_head_dty.
+
+  simpl; apply in_tail_dty;
+    auto.
+Qed.
+
+Lemma struct_contains_wf' :
+  forall Sig G t, Sig en G vdash t wf_t ->
+           forall s, s cont_w t ->
+                Sig en t::G vdash [c_ (length G) /s 0]s wf_s.
+Proof.
+  intros.
+  inversion H0;
+    subst.
+  inversion H;
+    subst.
+  eapply in_dty_wf; eauto.
+  apply subst_in_dty;
+    auto.
+Qed.
+
+Lemma struct_contains_wf :
+  forall Sig G t, Sig en G vdash t wf_t ->
+           forall s, s cont_w t ->
+                forall p, Sig en G vdash p pathType t ->
+                     Sig en t::G vdash [p /s 0]s wf_s.
+Proof.
+  intros.
   
   
 Qed.
+  
