type_members/ftfjp2018/coq/definitions.v
@@ -780,32 +780,6 @@ Scheme has_mut_ind := Induction for has Sort Prop
 
 Combined Scheme has_contains_mutind from has_mut_ind, contains_mut_ind.
 
-Reserved Notation "Sig 'en' G 'vdash' p 'ni_w' s" (at level 80).
-Reserved Notation "Sig 'en' G 'vdash' s 'cont_w' t" (at level 80).
-
-
-Inductive wf_contains : env -> env -> ty -> decl_ty -> Prop :=
-| cont_wf : forall Sig G ss s, in_dty s ss ->
-                        Sig en G vdash s cont_w (str ss)
-where "Sig 'en' G 'vdash' s 'cont_w' t" := (wf_contains Sig G t s).
-
-
-Inductive wf_has : env -> env -> exp -> decl_ty -> Prop :=
-| h_struct : forall Sig G p ss s, Sig en G vdash p pathType (str ss) ->
-                           Sig en G vdash s cont_w (str ss) ->
-                           Sig en G vdash p ni_w ([p /s 0] s)
-| h_upper : forall Sig G p p' l' t s, Sig en G vdash p pathType (sel p' l') ->
-                               Sig en G vdash p' ni_w (type l' ext t) ->
-                               Sig en G vdash (p cast t) ni_w s ->
-                               Sig en G vdash p ni_w s
-| h_equal : forall Sig G p p' l' t s, Sig en G vdash p pathType (sel p' l') ->
-                               Sig en G vdash p' ni_w (type l' eqt t) ->
-                               Sig en G vdash (p cast t) ni_w s ->
-                               Sig en G vdash p ni_w s
-where "Sig 'en' G 'vdash' p 'ni_w' s" := (wf_has Sig G p s).
-                                           
-
-Hint Constructors wf_has wf_contains.
 
 Reserved Notation "Sig 'en' G1 'vdash' t1 '<;' t2 'dashv' G2" (at level 80).
 Reserved Notation "Sig 'en' G1 'vdash' d1 '<;;' d2 'dashv' G2" (at level 80).
